fairness/lm_rules/fuel_step.v
@@ -3,8 +3,8 @@ From iris.proofmode Require Import tactics.
 From trillium.fairness Require Import fairness fuel fuel_ext resources partial_ownership.
 
 
-Section FuelStep.
-  Context `{LM: LiveModel G M LSI_True}.
+Section FuelDropStep.
+  Context `{LM: LiveModel G M LSI}.
   Context `{Countable G}.
   Context {Σ : gFunctors}.
   Context {fG: fairnessGS LM Σ}.
@@ -82,6 +82,258 @@ Section FuelStep.
     apply _.
   Qed.
 
+  (* TODO: move, generalize, upstream? *)
+  Lemma map_filter_diff_simpl (m: gmap (fmrole M) G) (R: gset (fmrole M)):
+    filter (fun '(k, _) => k ∈ dom m ∖ R) m = filter (fun '(k, _) => k ∉ R) m.
+  Proof. 
+    apply map_filter_ext. intros.
+    rewrite elem_of_difference elem_of_dom. set_solver. 
+  Qed.
+
+  (* Lemma frag_model_LSI s: *)
+  (* frag_model_is s -∗ ⌜ LSI ( ⌝ *)
+
+  Lemma actual_update_no_step_enough_fuel_drop
+  (δ1: LM) rem
+  (* c1 c2 *)
+  s fs ζ:
+    (dom fs ≠ ∅) ->
+    (live_roles _ δ1) ∩ rem = ∅ →
+    rem ⊆ dom fs →
+    fuel_drop_preserves_LSI s rem (LSI := LSI) ->
+    (* locale_step c1 (Some ζ) c2 -> *)
+    has_fuels_S ζ fs -∗ 
+    partial_model_is s -∗ 
+    model_state_interp δ1
+    ==∗ ∃ δ2,
+        ⌜ lm_ls_trans LM δ1 (Silent_step ζ) δ2 ⌝ ∗
+        has_fuels ζ (fs ⇂ (dom fs ∖ rem)) ∗
+        partial_model_is s ∗ 
+        model_state_interp δ2 ∗
+        ⌜ ls_tmap δ2 (LM := LM) = <[ζ:=dom fs ∖ rem]> (ls_tmap δ1 (LM := LM)) ⌝. 
+  Proof.
+    iIntros "%HnotO %Holdroles %Hincl %PRES Hf ST Hmod".
+    (* destruct c2 as [tp2 σ2]. *)
+    destruct (set_choose_L _ HnotO) as [??].
+    iDestruct (has_fuel_in with "Hf Hmod") as %Hxdom; eauto.
+    iDestruct (has_fuel_fuel with "Hf Hmod") as "%Hfuel"; eauto.
+    (* iDestruct (model_state_interp_tids_smaller with "Hmod") as %Hζs. *)
+    pose proof (ls_inv δ1) as LSI1. 
+    iDestruct "Hmod" as "(%FR & Hfuel & Hamapping & HFR & Hmodel & %HFR)".
+    iAssert (⌜ ls_tmap δ1 (LM := LM) !! ζ = Some (dom fs) ⌝)%I as %TMAP1.
+    { iDestruct "Hf" as "[MAP _]". simpl.
+      rewrite dom_fmap. 
+      iApply (frag_mapping_same with "Hamapping MAP"). }
+    unfold has_fuels_S.
+    simpl in *.
+
+    set new_dom := ((dom (ls_fuel δ1) ∪ dom fs) ∖ rem).
+    set new_mapping := ls_mapping δ1 ⇂ new_dom.
+
+    assert (dom (fuel_apply (filter (λ '(k, _), k ∈ dom fs ∖ rem) fs) (ls_fuel δ1)
+                   ((dom (ls_fuel δ1) ∪ dom fs) ∖ rem)) = new_dom) as Hnewdom.
+    { rewrite /fuel_apply map_imap_dom_eq ?dom_gset_to_gmap //.
+      intros ρ0 _ Hindom.
+      case_decide as Hninf; [by apply elem_of_dom|].
+      apply elem_of_difference in Hindom as [Hin1 ?].
+      apply elem_of_union in Hin1 as [?|Hin2]; first by apply elem_of_dom.
+      exfalso. apply Hninf. apply elem_of_dom in Hin2 as [f ?].
+      eapply elem_of_dom_2. rewrite map_filter_lookup_Some. split =>//.
+      apply elem_of_difference; split =>//. by eapply elem_of_dom_2. }
+
+    assert (Hsamedoms: dom new_mapping =
+                       dom (fuel_apply (fs ⇂ (dom fs ∖ rem))
+                                       (ls_fuel δ1)
+                                       ((dom (ls_fuel δ1) ∪ dom fs) ∖ rem))).
+    { rewrite /new_mapping /new_dom. unfold fuel_apply.
+      assert (dom fs ⊆ dom δ1.(ls_fuel)) as Hdom_le.
+      { intros ρ Hin. rewrite elem_of_dom Hfuel; last set_solver.
+        apply elem_of_dom in Hin as [? Hin]. rewrite lookup_fmap Hin //=. }
+      rewrite map_imap_dom_eq; last first.
+      { intros ρ _ Hin. rewrite dom_gset_to_gmap in Hin.
+        case_decide; [by apply elem_of_dom|].
+        apply elem_of_dom. set_solver +Hin Hdom_le. }
+      rewrite dom_domain_restrict ?dom_gset_to_gmap ?ls_same_doms //.
+      set_solver +Hdom_le. }
+    assert (Hfueldom: live_roles _ δ1 ⊆
+     dom (fuel_apply (fs ⇂ (dom fs ∖ rem))
+                     (ls_fuel δ1)
+                     ((dom (ls_fuel δ1) ∪ dom fs) ∖ rem))).
+    { rewrite /fuel_apply Hnewdom.
+      intros ρ Hin. apply elem_of_difference; split;
+        [apply ls_fuel_dom in Hin; set_solver +Hin|
+          set_solver -Hnewdom Hsamedoms]. }
+    iMod (update_has_fuels_no_step ζ (S <$> fs) (fs ⇂ (dom fs ∖ rem)) with "[Hf] [Hfuel] [Hamapping]") as "(Hafuels&Hfuels&Hamapping)" =>//.
+    { rewrite -dom_empty_iff_L. set_solver -Hnewdom Hsamedoms Hfueldom. }
+    { rewrite dom_domain_restrict; set_solver -Hnewdom Hsamedoms Hfueldom. }
+    rewrite dom_domain_restrict; [| set_solver]. 
+    iModIntro. 
+
+    pose proof (ls_mapping_tmap_corr δ1 (LM := LM)) as Hminv1. 
+    assert (dom fs ⊆ dom (ls_mapping δ1)) as INCL. 
+    { apply elem_of_subseteq. intros ρ' [f IN]%elem_of_dom.              
+      red in Hminv1. eapply elem_of_dom.
+      red. exists ζ. apply Hminv1. eexists. split; eauto.
+      eapply elem_of_dom. set_solver. }
+    assert (new_dom = dom (ls_mapping δ1) ∖ rem) as NEW_DOM. 
+    { rewrite /new_dom.
+      apply set_eq. intros.
+      pose proof (ls_same_doms δ1). 
+      destruct (decide (x ∈ rem)); [set_solver| ].      
+      destruct (decide (x ∈ dom (ls_mapping δ1))); set_solver. }
+    assert (maps_inverse_match new_mapping (<[ζ:=dom fs ∖ rem]>
+      (ls_tmap δ1 (LM := LM))
+           )) as MATCH.
+    { clear -Hxdom Hminv1 Hincl.
+      subst new_mapping new_dom. 
+      rewrite -ls_same_doms.
+      apply mim_fuel_helper; auto. }
+
+    (* TODO: doing this explicitly to avoid saving explicit proof terms
+       (parameters of build_LS_ext)
+       which otherwise critically slow down subsequent proofs *)
+    assert ( ∀ (τ1 τ2 : G) (S1 S2 : gset (fmrole M)),
+               τ1 ≠ τ2
+               → <[ζ:=dom fs ∖ rem]> (ls_tmap δ1) !! τ1 = Some S1
+               → <[ζ:=dom fs ∖ rem]> (ls_tmap δ1) !! τ2 = Some S2 → S1 ## S2) as DISJ2. 
+    { clear -TMAP1 tmap_disj. intros.
+      eapply tmap_update_subset_disjoint.
+      { red. apply (ls_tmap_disj δ1). }
+      2: eauto. 
+      2: apply H1. 2: apply H2.
+      intros ?? L%lookup_insert_Some.
+      destruct L as [[-> <-]| [? ?]].
+      all: eexists; split; eauto; set_solver. }
+
+    set (new_fuels := fuel_apply (filter (λ '(k, _), k ∈ dom fs ∖ rem) fs)
+           (ls_fuel δ1) ((dom (ls_fuel δ1) ∪ dom fs) ∖ rem)). 
+    assert ( ∀ ρ : fmrole M, ρ ∈ dom new_fuels
+    ↔ (∃ (τ : G) (R : gset (fmrole M)),
+         <[ζ:=dom fs ∖ rem]> (ls_tmap δ1) !! τ = Some R ∧ ρ ∈ R)) as TMAP_DOM2. 
+    { intros.
+      rewrite -Hsamedoms.
+      rewrite /new_mapping. 
+      erewrite dom_domain_restrict; [| set_solver]. 
+      rewrite NEW_DOM.
+      apply fuel_step_ls_tmap_dom; auto. }
+
+    iAssert (⌜ ls_under δ1 = s ⌝)%I as "%ST_EQ".
+    { iApply (model_agree with "Hmodel ST"). }
+    assert (LSI δ1 (ls_mapping_impl (<[ζ:=dom fs ∖ rem]> (ls_tmap δ1))) new_fuels) as LSI2.
+    { erewrite (maps_inverse_match_uniq1 (ls_mapping_impl _)); eauto.
+      2: { apply ls_mapping_tmap_corr_impl. apply DISJ2. }
+      subst new_mapping new_dom.
+      replace (dom (ls_fuel δ1) ∪ dom fs) with (dom (ls_fuel δ1)). 
+      2: { rewrite -ls_same_doms. set_solver. }
+      move PRES at bottom. red in PRES.
+      rewrite -ls_same_doms. rewrite map_filter_diff_simpl.
+      rewrite -ST_EQ in PRES. eapply PRES. eauto. }
+      
+    (* (* assert (forall s m f, LSI_True s m f) as mk_LT. *) *)
+    (* (* { intros. rewrite /LSI_True.  *) *)
+    (* assert (LSI s new_mapping new_fuels) as LSI2.  *)
+    (* { assert (dom (ls_fuel δ1) ∪ dom fs = dom (ls_fuel δ1)) as FUELS'.  *)
+    (*   { rewrite -ls_same_doms. set_solver. } *)
+    (*   subst new_mapping new_dom. rewrite FUELS'. *)
+    (*   move PRES at bottom. red in PRES. *)
+    (*   rewrite -ls_same_doms. rewrite map_filter_diff_simpl. *)
+    (*   eapply PRES. rewrite -ST_EQ. eauto. } *)
+
+
+    fold new_fuels in Hfueldom. 
+    iExists (build_LS_ext (ls_under δ1) _ Hfueldom (<[ζ:=dom fs ∖ rem]> (ls_tmap δ1 (LM := LM))) TMAP_DOM2 DISJ2 LSI2 (LM := LM)).
+
+    (* remember (build_LS_ext _ _ _ _ _ _) as δ2.  *)
+    simpl.
+    iSplit; last first.
+    { rewrite (dom_fmap_L _ fs). iFrame "Hfuels". 
+      (* rewrite /maps_inverse_match //=. *)
+      rewrite /model_state_interp. 
+      rewrite build_LS_ext_spec_st build_LS_ext_spec_fuel build_LS_ext_spec_tmap.
+      iFrame.
+      iSplitL; [| done]. 
+      assert (dom fs ⊆ dom (ls_fuel $ δ1)).
+      { intros ρ Hin. setoid_rewrite dom_fmap in Hxdom.
+        specialize (Hxdom ρ). rewrite -ls_same_doms. apply elem_of_dom. exists ζ.
+        by apply Hxdom. }
+      iExists _. iFrame. 
+      iSplit.
+      { subst new_fuels. 
+        iApply (auth_fuel_is_proper with "Hafuels"). f_equiv.
+        (* rewrite dom_domain_restrict; last set_solver -Hnewdom Hsamedoms Hfueldom. *)
+        replace (dom fs ∖ (dom fs ∖ rem)) with rem; [set_solver +|].
+        rewrite -leibniz_equiv_iff. intros ρ. split; [set_solver -Hnewdom Hsamedoms Hfueldom|].
+        intros [? [?|?]%not_elem_of_difference]%elem_of_difference =>//. }
+      iPureIntro.
+      (* split. *)
+      (* - intros. eapply tids_dom_restrict_mapping; eauto.  *)
+      - rewrite Hnewdom /new_dom. apply elem_of_equiv_empty_L. intros ρ [Hin1 Hin2]%elem_of_intersection.
+        assert (ρ ∈ dom (ls_fuel δ1))
+               by set_solver -Hnewdom Hsamedoms Hfueldom.
+        set_solver -Hnewdom Hsamedoms Hfueldom. }
+        
+    iPureIntro.
+    (* split; [split; [|split; [|split; [|split]]]|] =>//. *)
+    repeat split; try done. 
+    - eexists. apply Hxdom. by rewrite dom_fmap.
+    - unfold fuel_decr. simpl.
+      rewrite (build_LS_ext_spec_fuel). 
+      intros ρ' Hin Hin' Hmustdec.
+      rewrite Hnewdom in Hin'.
+
+      inversion Hmustdec; simplify_eq.
+      + have Hinfs: ρ' ∈ dom (S <$> fs) by set_solver.
+        rewrite map_lookup_imap Hfuel // lookup_fmap. rewrite dom_fmap in Hinfs.
+        rewrite lookup_gset_to_gmap option_guard_True //=.
+
+        pose proof Hinfs as Hinfs'. apply elem_of_dom in Hinfs' as [f Heqf].
+        assert (filter (λ '(k, _), k ∈ dom fs ∖ rem) fs !! ρ' = Some f) as Heqfilter.
+        { rewrite map_filter_lookup Heqf /= option_guard_True //. set_solver -Hnewdom Hsamedoms Hfueldom Hmustdec. }
+        rewrite decide_True // ?Heqfilter ?lookup_fmap ?Heqf /=; last by eapply elem_of_dom_2. lia.
+      + erewrite build_LS_ext_spec_mapping in Hneqtid; [| by eauto].
+        rewrite /= /new_mapping map_filter_lookup in Hneqtid.
+        pose proof Hin as Hin2. rewrite -ls_same_doms in Hin2. apply elem_of_dom in Hin2 as [f Hf].
+        rewrite Hf /= option_guard_True // in Hneqtid.
+    - intros ρ' Hin. simpl. destruct (decide (ρ' ∈ rem)) as [Hin'|Hnin'].
+      + right. right. 
+        split; last set_solver -Hnewdom Hsamedoms Hfueldom.
+        rewrite build_LS_ext_spec_fuel. 
+        rewrite /fuel_apply map_imap_dom_eq ?dom_gset_to_gmap; first set_solver.
+        intros ρ0 _ Hin0. 
+        case_decide as Hnin; [by apply elem_of_dom|].
+        apply elem_of_difference in Hin0 as [Hin1 ?].
+        apply elem_of_union in Hin1 as [?|Hin2]; first by apply elem_of_dom.
+        exfalso. apply Hnin. apply elem_of_dom in Hin2 as [f ?].
+        eapply elem_of_dom_2. rewrite map_filter_lookup_Some. split =>//.
+        apply elem_of_difference; split =>//. by eapply elem_of_dom_2.
+      + left.
+        rewrite build_LS_ext_spec_fuel. 
+        rewrite map_lookup_imap lookup_gset_to_gmap option_guard_True //=;
+                      last set_solver -Hnewdom Hsamedoms Hfueldom.
+        apply elem_of_dom in Hin as [f Hf].
+        case_decide as Hin; [|by rewrite !Hf //=].
+        apply elem_of_dom in Hin as [f' Hf']. rewrite Hf'.
+        apply map_filter_lookup_Some in Hf' as [Hfs Hf'].
+        rewrite Hfuel ?lookup_fmap ?Hfs /=; [lia |].
+        rewrite dom_fmap; set_solver -Hnewdom Hsamedoms Hfueldom.
+    - rewrite build_LS_ext_spec_fuel. 
+      rewrite Hnewdom. assert (dom fs ⊆ dom $ ls_fuel δ1);
+        last set_solver -Hnewdom Hsamedoms Hfueldom.
+      intros ρ Hin. apply elem_of_dom.
+      rewrite Hfuel ?dom_fmap // -elem_of_dom dom_fmap //.
+    - by rewrite build_LS_ext_spec_st.   
+  Qed. 
+
+End FuelDropStep. 
+
+
+(* TODO: remove lots of duplication between two rules *)
+Section FuelStep.
+  Context `{LM: LiveModel G M LSI_True}.
+  Context `{Countable G}.
+  Context {Σ : gFunctors}.
+  Context {fG: fairnessGS LM Σ}.
+
   Lemma actual_update_no_step_enough_fuel
   (δ1: LM) rem
   (* c1 c2 *)
@@ -96,7 +348,7 @@ Section FuelStep.
         has_fuels ζ (fs ⇂ (dom fs ∖ rem)) ∗
         model_state_interp δ2 ∗
         ⌜ ls_tmap δ2 (LM := LM) = <[ζ:=dom fs ∖ rem]> (ls_tmap δ1 (LM := LM)) ⌝. 
-Proof.
+  Proof.
     iIntros "%HnotO %Holdroles %Hincl Hf Hmod".
     (* destruct c2 as [tp2 σ2]. *)
     destruct (set_choose_L _ HnotO) as [??].
@@ -180,7 +432,7 @@ Proof.
                τ1 ≠ τ2
                → <[ζ:=dom fs ∖ rem]> (ls_tmap δ1) !! τ1 = Some S1
                → <[ζ:=dom fs ∖ rem]> (ls_tmap δ1) !! τ2 = Some S2 → S1 ## S2) as DISJ2. 
-    { clear -TMAP1 tmap_disj. intros.
+    { clear -TMAP1. intros.
       eapply tmap_update_subset_disjoint.
       { red. apply (ls_tmap_disj δ1). }
       2: eauto. 
