fairness/lm_steps_gen.v
@@ -1,0 +1,145 @@
+From iris.algebra Require Import auth gmap gset excl.
+From iris.proofmode Require Import tactics.
+From trillium.fairness Require Import execution_model.
+From trillium.fairness Require Import fairness fuel fuel_ext. 
+From trillium.fairness Require Import partial_ownership.
+
+
+Section LMSteps.
+  Context `{iLM: LiveModel G iM LSI}.
+  Context `{EM: ExecutionModel Λ M}.
+  Context `{eGS: em_GS Σ}. 
+  Context `{invGS_gen HasNoLc Σ}.
+  Context `{Countable (locale Λ)}. 
+  Context {PMPP: @PartialModelPredicatesPre (locale Λ) _ _ Σ iM}.
+
+  Let update_no_step_enough_fuel_drop_def (extr : execution_trace Λ) 
+      (auxtr : auxiliary_trace M) 
+      (c2 : cfg Λ) s (fs : gmap (fmrole iM) nat) rem (ζ : locale Λ)
+      `(dom fs ≠ ∅)
+      `((live_roles _ s) ∩ rem = ∅)
+      `(rem ⊆ dom fs)
+      `(locale_step (trace_last extr) (Some ζ) c2)
+      `(fuel_drop_preserves_LSI s rem (LSI := LSI))
+    : iProp Σ :=
+    has_fuels ζ (S <$> fs) -∗
+    partial_model_is s -∗
+    em_msi (trace_last extr) (trace_last auxtr) (em_GS0 := eGS) ==∗
+    ∃ (δ2 : M) (ℓ : mlabel M),
+      ⌜em_valid_state_evolution_fairness (extr :tr[ Some ζ ]: c2)
+      (auxtr :tr[ ℓ ]: δ2)⌝ ∗
+      has_fuels ζ (filter (λ '(k, _), k ∈ dom fs ∖ rem) fs) ∗
+      partial_model_is s ∗
+      em_msi c2 δ2 (em_GS0 := eGS).
+  
+  Let update_no_step_enough_fuel_keep_def (extr : execution_trace Λ)
+      (auxtr : auxiliary_trace M)
+      (c2 : cfg Λ) (fs : gmap (fmrole iM) nat) (ζ : locale Λ)
+      `(dom fs ≠ ∅)
+      `(locale_step (trace_last extr) (Some ζ) c2)
+      `(fuel_reorder_preserves_LSI (LSI := LSI))
+    : iProp Σ :=
+    has_fuels ζ (S <$> fs) -∗
+    em_msi (trace_last extr) (trace_last auxtr) (em_GS0 := eGS) ==∗
+    ∃ (δ2 : M) (ℓ : mlabel M),
+      ⌜em_valid_state_evolution_fairness (extr :tr[ Some ζ ]: c2)
+      (auxtr :tr[ ℓ ]: δ2)⌝ ∗
+      has_fuels ζ (filter (λ '(k, _), k ∈ dom fs) fs) ∗
+      em_msi c2 δ2 (em_GS0 := eGS).
+  
+  Let update_fork_split_def (R1 R2: gset (fmrole iM)) tp1 tp2
+       (fs: gmap (fmrole iM) nat)
+        (extr : execution_trace Λ)
+        (auxtr: auxiliary_trace M) ζ efork σ1 σ2
+          `(R1 ## R2)
+          `(fs ≠ ∅)
+          `(R1 ∪ R2 = dom fs)
+          `(fuel_reorder_preserves_LSI (LSI := LSI))
+         `(trace_last extr = (tp1, σ1))
+          `(locale_step (tp1, σ1) (Some ζ) (tp2, σ2))
+          `((∃ tp1', tp2 = tp1' ++ [efork] ∧ length tp1' = length tp1)): iProp Σ :=
+     has_fuels ζ (S <$> fs) -∗
+     em_msi (trace_last extr) (trace_last auxtr) (em_GS0 := eGS) ==∗
+     ∃ δ2 ℓ, has_fuels (locale_of tp1 efork) (fs ⇂ R2) ∗
+             has_fuels ζ (fs ⇂ R1) ∗
+             (partial_mapping_is {[ locale_of tp1 efork := ∅ ]} -∗
+              em_thread_post (locale_of tp1 efork) (em_GS0 := eGS)) ∗
+             em_msi (tp2, σ2) δ2 (em_GS0 := eGS) ∧ 
+             ⌜em_valid_state_evolution_fairness (extr :tr[Some ζ]: (tp2, σ2)) (auxtr :tr[ℓ]: δ2)⌝.
+
+  Let update_step_still_alive_def
+      (extr : execution_trace Λ)
+      (auxtr: auxiliary_trace M)
+       tp1 tp2 σ1 σ2
+       (s1 s2: iM)
+       (fs1 fs2: gmap (fmrole iM) nat)
+      ρ (δ1 : M) ζ fr1 fr_stash
+       (Einvs: coPset)
+     `((live_roles _ s2 ∖ live_roles _ s1) ⊆ fr1)
+     `(fr_stash ⊆ dom fs1)
+     `((live_roles _ s1) ∩ (fr_stash ∖ {[ ρ ]}) = ∅)
+     `(dom fs2 ∩ fr_stash = ∅)
+    `(trace_last extr = (tp1, σ1))
+    `(trace_last auxtr = δ1)
+     `(locale_step (tp1, σ1) (Some ζ) (tp2, σ2))
+     `(fmtrans _ s1 (Some ρ) s2)
+     `(valid_new_fuelmap fs1 fs2 s1 s2 ρ (LM := iLM))
+     `(model_step_preserves_LSI s2 fs1 fs2 (LSI := LSI))
+    : iProp Σ :=
+      has_fuels ζ fs1 -∗
+      partial_model_is s1 -∗
+      em_msi (tp1, σ1) δ1 (em_GS0 := eGS) -∗
+      partial_free_roles_are fr1
+      ={ Einvs }=∗
+      ∃ (δ2: M) ℓ,
+      ⌜em_valid_state_evolution_fairness (extr :tr[Some ζ]: (tp2, σ2)) (auxtr :tr[ℓ]: δ2)⌝ ∗
+      has_fuels ζ fs2 ∗
+      partial_model_is s2 ∗
+      em_msi (tp2, σ2) δ2 (em_GS0 := eGS)∗
+      partial_free_roles_are (fr1 ∖ (live_roles _ s2 ∖ live_roles _ s1) ∪ fr_stash).
+
+    (* TODO: where to place it? *)
+    (* Let partial_free_roles_fuels_disj_def δ fr fs tid: iProp Σ := *)
+    (*     partial_msi δ -∗ partial_free_roles_are fr -∗ has_fuels tid fs -∗ ⌜ fr ## dom fs ⌝. *)
+
+    Let LM_steps_gen_def (Einvs: coPset): iProp Σ := □ (
+          (∀ extr auxtr c2 s fs rem ζ NE NL RD STEP PRES, update_no_step_enough_fuel_drop_def extr auxtr c2 s fs rem ζ NE NL RD STEP PRES) ∗
+          (∀ extr auxtr c2 fs ζ NE STEP PRES, update_no_step_enough_fuel_keep_def extr auxtr c2 fs ζ NE STEP PRES) ∗
+          (∀ R1 R2 tp1 tp2 fs extr auxtr ζ efork σ1 σ2 DISJ NE DOM PRES LAST STEP POOL, 
+update_fork_split_def R1 R2 tp1 tp2 fs extr auxtr ζ efork σ1 σ2 DISJ NE DOM PRES LAST STEP POOL) ∗
+          (∀ extr auxtr tp1 tp2 σ1 σ2 s1 s2 fs1 fs2 ρ δ1 ζ fr1 fr_stash
+             LR STASH STASH' STASH'' LAST1 LAST2 STEP STEP' VFM PRES,
+              update_step_still_alive_def extr auxtr tp1 tp2 σ1 σ2 s1 s2 fs1 fs2 ρ δ1 ζ fr1 fr_stash Einvs LR STASH STASH' STASH'' LAST1 LAST2 STEP STEP' VFM PRES)
+).  
+
+    Definition LM_steps_gen Einvs: iProp Σ := LM_steps_gen_def Einvs.
+
+    Lemma Build_LM_steps_gen Einvs:
+      LM_steps_gen_def Einvs ⊢ LM_steps_gen Einvs.
+    Proof. done. Qed. 
+
+    Global Instance LM_steps_gen_pers: forall Einvs, Persistent (LM_steps_gen Einvs).
+    Proof. apply _. Qed.
+
+    Lemma update_no_step_enough_fuel_drop_gen {Einvs} extr auxtr c2 s fs rem ζ NE NL RD STEP PRES: 
+      LM_steps_gen Einvs ⊢ update_no_step_enough_fuel_drop_def extr auxtr c2 s fs rem ζ NE NL RD STEP PRES. 
+    Proof. by iIntros "(?&?&?&?)". Qed.
+
+    Lemma update_no_step_enough_fuel_keep_gen {Einvs} extr auxtr c2 fs ζ NE STEP PRES: 
+      LM_steps_gen Einvs ⊢ update_no_step_enough_fuel_keep_def extr auxtr c2 fs ζ NE STEP PRES. 
+    Proof. by iIntros "(?&?&?&?)". Qed.
+
+    Lemma update_fork_split_gen {Einvs} R1 R2 tp1 tp2 fs extr auxtr ζ efork σ1 σ2 DISJ NE DOM PRES LAST STEP POOL: 
+      LM_steps_gen Einvs ⊢ update_fork_split_def R1 R2 tp1 tp2 fs extr auxtr ζ efork σ1 σ2 DISJ NE DOM PRES LAST STEP POOL. 
+    Proof. by iIntros "(?&?&?&?)". Qed.
+
+    Lemma update_step_still_alive_gen {Einvs} extr auxtr tp1 tp2 σ1 σ2 s1 s2 fs1 fs2 ρ δ1 ζ fr1 fr_stash
+             LR STASH STASH' STASH'' LAST1 LAST2 STEP STEP' VFM PRES:
+      LM_steps_gen Einvs ⊢ update_step_still_alive_def extr auxtr tp1 tp2 σ1 σ2 s1 s2 fs1 fs2 ρ δ1 ζ fr1 fr_stash Einvs
+             LR STASH STASH' STASH'' LAST1 LAST2 STEP STEP' VFM PRES.
+    Proof. by iIntros "(?&?&?&?)". Qed. 
+
+
+    Global Opaque LM_steps_gen.
+
+End LMSteps.
